veric_ext/SeparationLogic.v
@@ -1,79 +1,46 @@
+Require Export RamifyCoq.msl_ext.seplog.
+Require Export RamifyCoq.msl_ext.log_normalize.
+Require Export RamifyCoq.msl_ext.alg_seplog.
+Require Export RamifyCoq.veric_ext.seplog.
 Require Import VST.veric.SeparationLogic.
-Require Import RamifyCoq.msl_ext.abs_addr.
-Require Import RamifyCoq.msl_ext.seplog.
-Require Import RamifyCoq.msl_ext.alg_seplog.
-Require Import RamifyCoq.veric_ext.seplog.
 
 Instance PSLveric: PreciseSepLog mpred := algPreciseSepLog compcert_rmaps.RML.R.rmap.
 Instance OSLveric: OverlapSepLog mpred := algOverlapSepLog compcert_rmaps.RML.R.rmap.
 Instance DSLveric: DisjointedSepLog mpred := algDisjointedSepLog compcert_rmaps.RML.R.rmap.
+Instance COSLveric: CorableOverlapSepLog mpred := algCorableOverlapSepLog compcert_rmaps.RML.R.rmap.
 
-Module Mapsto.
-Section Mapsto.
+Instance LiftPreciseSepLog' T {ND: NatDed T}{SL: SepLog T}{PSL: PreciseSepLog T} :
+           PreciseSepLog (LiftEnviron T) := LiftPreciseSepLog _ _.
+Instance LiftOverlapSepLog' T {ND: NatDed T}{SL: SepLog T}{PSL: PreciseSepLog T}{OSL: OverlapSepLog T} :
+           OverlapSepLog (LiftEnviron T) := LiftOverlapSepLog _ _.
+Instance LiftDisjointedSepLog' T {ND: NatDed T}{SL: SepLog T}{PSL: PreciseSepLog T}{OSL: OverlapSepLog T}{DSL: DisjointedSepLog T} :
+           DisjointedSepLog (LiftEnviron T) := LiftDisjointedSepLog _ _.
 
-Definition adr_conflict (a1 a2 : val * type) : bool :=
-  match a1, a2 with
-  | (p1, t1), (p2, t2) => 
-    if (pointer_range_overlap_dec p1 (BV_sizeof t1) p2 (BV_sizeof t2)) then true else false
-  end.
+Global Opaque PSLveric OSLveric DSLveric COSLveric.
 
-Instance AbsAddr_veric : AbsAddr.
-  apply (mkAbsAddr (val * type) val adr_conflict); intros; unfold adr_conflict in *; destruct p1, p2.
-  + destruct (pointer_range_overlap_dec v (BV_sizeof t) v0 (BV_sizeof t0)); subst;
-    destruct (pointer_range_overlap_dec v0 (BV_sizeof t0) v (BV_sizeof t)); subst; auto;
-    pose proof pointer_range_overlap_comm v (BV_sizeof t) v0 (BV_sizeof t0);
-    tauto.
-  + destruct (pointer_range_overlap_dec v (BV_sizeof t) v0 (BV_sizeof t0)); auto.
-    destruct (pointer_range_overlap_isptr _ _ _ _ p).
-    destruct (zlt 0 (BV_sizeof t)).
-    - assert (pointer_range_overlap v (BV_sizeof t) v (BV_sizeof t))
-        by (apply pointer_range_overlap_refl; auto; omega).
-      destruct (pointer_range_overlap_dec v (BV_sizeof t) v (BV_sizeof t)); [congruence | tauto].
-    - apply pointer_range_overlap_non_zero in p.
-      omega.
-Defined.
+Local Open Scope logic.
 
-Instance MSLveric sh: MapstoSepLog AbsAddr_veric (fun pt v => let (p, t) := pt in mapsto sh t p v).
-Proof.
-  apply mkMapstoSepLog.
-  intros [p t].
-  apply exp_mapsto_precise.
-Defined.
+Lemma exp_mapsto_precise: forall sh t p, precise (EX v: val, mapsto sh t p v).
+Proof. exact exp_mapsto_precise. Qed.
 
-Instance sMSLveric sh: StaticMapstoSepLog AbsAddr_veric (fun pt v => let (p, t) := pt in mapsto sh t p v).
-Proof.
-  apply mkStaticMapstoSepLog.
-  + intros [p t] v ?.
-    unfold addr_empty in H; simpl in H.
-    destruct (pointer_range_overlap_dec p (BV_sizeof t) p (BV_sizeof t)); [congruence |].
-    unfold mapsto.
-    destruct (access_mode t) eqn:?H; try apply FF_left.
-    destruct (type_is_volatile t), p; try apply FF_left.
-    assert (pointer_range_overlap (Vptr b i) (BV_sizeof t) (Vptr b i) (BV_sizeof t)); [| tauto].
-    apply pointer_range_overlap_refl.
-    - simpl; tauto.
-    - eapply BV_sizeof_pos; eauto.
-    - eapply BV_sizeof_pos; eauto.
-  + intros [p1 t1] [p2 t2] v1 v2 ?.
-    apply mapsto_conflict with (PTree.empty _).
-    apply pointer_range_overlap_BV_sizeof.
-    simpl in H.
-    destruct (pointer_range_overlap_dec p1 (BV_sizeof t1) p2 (BV_sizeof t2)); [auto | congruence].
-  + intros [p1 t1] [p2 t2] ?.
-    simpl in H.
-    destruct (pointer_range_overlap_dec p1 (BV_sizeof t1) p2 (BV_sizeof t2)); [congruence |].
-    destruct (pointer_range_overlap_dec p1 (sizeof (PTree.empty _) t1) p2 (sizeof (PTree.empty _) t2)).
-    - apply pointer_range_overlap_sizeof with (sh := sh) in p.
-      destruct p as [? | [? | ?]].
-      * tauto.
-      * eapply disj_derives; [exact H0 | apply derives_refl |].
-        pose proof log_normalize.FF_disj.
-        simpl in H1; apply H1.
-      * eapply disj_derives; [apply derives_refl | exact H0 |].
-        pose proof log_normalize.disj_FF.
-        simpl in H1; apply H1.
-    - apply disj_mapsto_ with (PTree.empty _); auto.
-Defined.
+Lemma disj_mapsto_: forall sh env t1 t2 p1 p2,
+  ~ pointer_range_overlap p1 (sizeof env t1) p2 (sizeof env t2) ->
+  disjointed (EX v1: val, mapsto sh t1 p1 v1) (EX v2: val, mapsto sh t2 p2 v2).
+Proof. exact disj_mapsto_. Qed.
 
-End Mapsto.
-End Mapsto.
+Lemma mapsto_conflict: forall sh env t1 t2 p1 p2 v1 v2,
+  pointer_range_overlap p1 (sizeof env t1) p2 (sizeof env t2) ->
+  mapsto sh t1 p1 v1 * mapsto sh t2 p2 v2 |-- FF.
+Proof. exact mapsto_conflict. Qed.
+
+Lemma memory_block_precise: forall sh p n, precise (memory_block sh n p).
+Proof. exact memory_block_precise. Qed.
+
+Lemma disj_memory_block: forall sh p1 n1 p2 n2, ~ pointer_range_overlap p1 n1 p2 n2 -> disjointed (memory_block sh n1 p1) (memory_block sh n2 p2).
+Proof. exact disj_memory_block. Qed.
+
+Lemma memory_block_conflict: forall sh p1 n1 p2 n2, pointer_range_overlap p1 n1 p2 n2 -> memory_block sh n1 p1 * memory_block sh n2 p2 |-- FF.
+Proof. exact memory_block_conflict. Qed.
+
+
+
