floyd_ext/DataatSL.v
@@ -1,0 +1,52 @@
+Require Import VST.floyd.base.
+Require Import VST.floyd.client_lemmas.
+Require Import VST.floyd.assert_lemmas.
+Require Import VST.floyd.type_induction.
+Require Import VST.floyd.nested_pred_lemmas.
+Require Import VST.floyd.nested_field_lemmas.
+Require Import VST.floyd.reptype_lemmas.
+Require Import VST.floyd.field_at.
+Require Import RamifyCoq.veric_ext.seplog.
+Require Import RamifyCoq.veric_ext.SeparationLogic.
+Require Import RamifyCoq.floyd_ext.MapstoSL.
+
+Local Open Scope logic.
+
+Section DataAtMSL.
+
+Context {cs: compspecs}.
+Context {csl: compspecs_legal cs}.
+
+Lemma exp_data_at_precise: forall sh t p,
+  precise (EX v: reptype t, data_at sh t v p).
+Proof.
+  intros.
+  apply derives_precise with (memory_block sh (sizeof cenv_cs t) p).
+  + apply exp_left; intro v.
+    apply data_at_memory_block; auto.
+  + apply seplog.memory_block_precise.
+Qed.
+
+Lemma disj_data_at: forall sh t1 t2 p1 p2,
+  ~ pointer_range_overlap p1 (sizeof cenv_cs t1) p2 (sizeof cenv_cs t2) ->
+  disjointed (EX v: reptype t1, data_at sh t1 v p1) (EX v: reptype t2, data_at sh t2 v p2).
+Proof.
+  intros.
+  eapply disj_derives; [| | apply disj_memory_block].
+  + apply exp_left; intro v.
+    apply data_at_memory_block.
+  + apply exp_left; intro v.
+    apply data_at_memory_block.
+  + auto.
+Qed.
+
+Lemma data_at_conflict: forall sh t1 t2 p1 p2 v1 v2,
+  pointer_range_overlap p1 (sizeof cenv_cs t1) p2 (sizeof cenv_cs t2) ->
+  data_at sh t1 v1 p1 * data_at sh t2 v2 p2 |-- FF.
+Proof.
+  intros.
+  eapply derives_trans; [apply sepcon_derives; apply data_at_memory_block |].
+  apply memory_block_conflict; auto.
+Qed.
+
+End DataAtMSL.
