floyd_ext/MapstoSL.v
@@ -1,0 +1,153 @@
+Require Import VST.floyd.base.
+Require Import VST.floyd.assert_lemmas.
+Require Import VST.floyd.client_lemmas.
+Require Import VST.floyd.nested_pred_lemmas.
+Require Import VST.floyd.mapsto_memory_block.
+
+Require Import RamifyCoq.msl_ext.abs_addr.
+Require Import RamifyCoq.msl_ext.seplog.
+Require Import RamifyCoq.msl_ext.log_normalize.
+Require Import RamifyCoq.veric_ext.SeparationLogic.
+
+Local Open Scope logic.
+
+Module Mapsto.
+Section Mapsto.
+
+Definition adr_conflict (a1 a2 : val * type) : bool :=
+  match a1, a2 with
+  | (p1, t1), (p2, t2) => 
+    if (pointer_range_overlap_dec p1 (BV_sizeof t1) p2 (BV_sizeof t2)) then true else false
+  end.
+
+Instance AA : AbsAddr.
+  apply (mkAbsAddr (val * type) val adr_conflict); intros; unfold adr_conflict in *; destruct p1, p2.
+  + destruct (pointer_range_overlap_dec v (BV_sizeof t) v0 (BV_sizeof t0)); subst;
+    destruct (pointer_range_overlap_dec v0 (BV_sizeof t0) v (BV_sizeof t)); subst; auto;
+    pose proof pointer_range_overlap_comm v (BV_sizeof t) v0 (BV_sizeof t0);
+    tauto.
+  + destruct (pointer_range_overlap_dec v (BV_sizeof t) v0 (BV_sizeof t0)); auto.
+    destruct (pointer_range_overlap_isptr _ _ _ _ p).
+    destruct (zlt 0 (BV_sizeof t)).
+    - assert (pointer_range_overlap v (BV_sizeof t) v (BV_sizeof t))
+        by (apply pointer_range_overlap_refl; auto; omega).
+      destruct (pointer_range_overlap_dec v (BV_sizeof t) v (BV_sizeof t)); [congruence | tauto].
+    - apply pointer_range_overlap_non_zero in p.
+      omega.
+Defined.
+
+Instance MSL sh: MapstoSepLog AA (fun pt v => let (p, t) := pt in mapsto sh t p v).
+Proof.
+  apply mkMapstoSepLog.
+  intros [p t].
+  apply exp_mapsto_precise.
+Defined.
+
+Instance sMSL sh: StaticMapstoSepLog AA (fun pt v => let (p, t) := pt in mapsto sh t p v).
+Proof.
+  apply mkStaticMapstoSepLog.
+  + intros [p t] v ?.
+    unfold addr_empty in H; simpl in H.
+    destruct (pointer_range_overlap_dec p (BV_sizeof t) p (BV_sizeof t)); [congruence |].
+    unfold mapsto.
+    destruct (access_mode t) eqn:?H; try apply FF_left.
+    destruct (type_is_volatile t), p; try apply FF_left.
+    assert (pointer_range_overlap (Vptr b i) (BV_sizeof t) (Vptr b i) (BV_sizeof t)); [| tauto].
+    apply pointer_range_overlap_refl.
+    - simpl; tauto.
+    - eapply BV_sizeof_pos; eauto.
+    - eapply BV_sizeof_pos; eauto.
+  + intros [p1 t1] [p2 t2] v1 v2 ?.
+    apply mapsto_conflict with (PTree.empty _).
+    apply pointer_range_overlap_BV_sizeof.
+    simpl in H.
+    destruct (pointer_range_overlap_dec p1 (BV_sizeof t1) p2 (BV_sizeof t2)); [auto | congruence].
+  + intros [p1 t1] [p2 t2] ?.
+    simpl in H.
+    destruct (pointer_range_overlap_dec p1 (BV_sizeof t1) p2 (BV_sizeof t2)); [congruence |].
+    destruct (pointer_range_overlap_dec p1 (sizeof (PTree.empty _) t1) p2 (sizeof (PTree.empty _) t2)).
+    - apply pointer_range_overlap_sizeof with (sh := sh) in p.
+      destruct p as [? | [? | ?]].
+      * tauto.
+      * eapply disj_derives; [exact H0 | apply derives_refl |].
+        pose proof log_normalize.FF_disj.
+        simpl in H1; apply H1.
+      * eapply disj_derives; [apply derives_refl | exact H0 |].
+        pose proof log_normalize.disj_FF.
+        simpl in H1; apply H1.
+    - apply disj_mapsto_ with (PTree.empty _); auto.
+Defined.
+
+End Mapsto.
+End Mapsto.
+
+Module MemoryBlock.
+Section MemoryBlock.
+
+Definition adr_conflict (a1 a2 : val * Z) : bool :=
+  match a1, a2 with
+  | (p1, n1), (p2, n2) => 
+    if (pointer_range_overlap_dec p1 n1 p2 n2) then true else false
+  end.
+
+Instance AA : AbsAddr.
+  apply (mkAbsAddr (val * Z) unit adr_conflict); intros; unfold adr_conflict in *; destruct p1, p2.
+  + destruct (pointer_range_overlap_dec v z v0 z0); subst;
+    destruct (pointer_range_overlap_dec v0 z0 v z); subst; auto;
+    pose proof pointer_range_overlap_comm v z v0 z0;
+    tauto.
+  + destruct (pointer_range_overlap_dec v z v0 z0); auto.
+    destruct (pointer_range_overlap_isptr _ _ _ _ p).
+    destruct (zlt 0 z).
+    - assert (pointer_range_overlap v z v z)
+        by (apply pointer_range_overlap_refl; auto; omega).
+      destruct (pointer_range_overlap_dec v z v z); [congruence | tauto].
+    - apply pointer_range_overlap_non_zero in p.
+      omega.
+Defined.
+
+Instance MSL sh: MapstoSepLog AA (fun pn v => let (p, n) := pn in memory_block sh n p).
+Proof.
+  apply mkMapstoSepLog.
+  intros [p n].
+  rewrite exp_unit.
+  apply memory_block_precise.
+Defined.
+
+Instance sMSL sh: StaticMapstoSepLog AA (fun pn v => let (p, n) := pn in memory_block sh n p).
+Proof.
+  apply mkStaticMapstoSepLog.
+  + intros [p n] v ?.
+    unfold addr_empty in H; simpl in H.
+    destruct (pointer_range_overlap_dec p n p n); [congruence |].
+    rewrite memory_block_isptr.
+    normalize.
+    destruct p; try inversion Pp.
+    destruct (zlt 0 n).
+    - assert (pointer_range_overlap (Vptr b i) n (Vptr b i) n); [| tauto].
+      apply pointer_range_overlap_refl; simpl; try tauto; omega.
+    - change memory_block with seplog.memory_block.
+      unfold seplog.memory_block.
+      rewrite nat_of_Z_neg by omega.
+      simpl.
+      change (predicates_hered.andp
+        (predicates_hered.prop (Int.unsigned i + n <= Int.modulus))
+        predicates_sl.emp) with (!! (Int.unsigned i + n <= Int.modulus) && emp)%logic.
+      apply andp_left2; auto.
+  + intros [p1 n1] [p2 n2] _ _ ?.
+    apply memory_block_conflict.
+    simpl in H.
+    destruct (pointer_range_overlap_dec p1 n1 p2 n2); [auto | congruence].
+  + intros [p1 n1] [p2 n2] ?.
+    simpl in H.
+    unfold mapsto_.
+    rewrite !exp_unit.
+    destruct (pointer_range_overlap_dec p1 n1 p2 n2); [congruence |].
+    destruct (pointer_range_overlap_dec p1 n1 p2 n2); [tauto |].
+    apply disj_memory_block; auto.
+Defined.
+
+End MemoryBlock.
+End MemoryBlock.
+
+
